typeclass/Util/spl_def.v
@@ -28,6 +28,9 @@ Import CKTransSPL.
 Import FeatureModelSPL.
 Import AssetMappingSPL.  
 
+  Variable c : Conf.
+  Axiom confs_dec : forall x y:set Conf, {x = y} + {x <> y}.
+  Axiom as_dec : forall x y: Asset, {x = y} + {x <> y}.
 
 
   Definition ArbitrarySPL: Type := FM * AM * CK.
@@ -37,22 +40,25 @@ Import AssetMappingSPL.
   Definition getFM_func (PL: ArbitrarySPL) : FM := fst ( fst PL).
   Definition getAM_func (PL: ArbitrarySPL) : AM := snd ( fst PL).
   Definition getCK_func (PL: ArbitrarySPL) : CK := snd PL.
-
+  Definition getCk_func ck : CK := ck.
 
   Definition wfPL_func (pl:ArbitrarySPL): Prop :=
     (forall c, set_In c (FMRef_Func (getFM_func pl)) ->
       wfProduct_ind (CKSem_func (getCK_func pl) (getAM_func pl) c)).
 
+
   (* Definition <Product line> *) 
-  Definition PL : Type := ArbitrarySPL.
+  Record PL: Type := {
+        pls:> ArbitrarySPL;
+        wfpl:> Prop }.
+
+  Variable pl pl1 pl2: PL.
+
   Definition plRefinement_func (pl1 pl2: PL): Prop :=
       (forall c1, set_In c1 (FMRef_Func (getFM_func pl1)) ->
         (exists c2, set_In c2 (FMRef_Func (getFM_func pl2)) /\
           ( assetRef_func (CKSem_func (getCK_func pl1) (getAM_func pl1) (c1)) 
               (CKSem_func (getCK_func pl2) (getAM_func pl2) (c2))))). 
-
-  Axiom confs_dec : forall x y:set Conf, {x = y} + {x <> y}.
-  Variable pl pl1 pl2: PL.
 
 
   Fixpoint genConf (AS : set Asset) : set Asset := 
@@ -75,7 +81,7 @@ Import AssetMappingSPL.
    | nil => nil
    | a1 :: x1 => filterAux pl AS a1 ++ filter pl AS x1
   end.
-  Variable c : Conf.
+
   
 
   Definition products_func (pl : PL): set Asset := 
@@ -87,7 +93,7 @@ Import AssetMappingSPL.
         (assetRef_func p1 p2))).
 
   Definition subsetProducts_func (pl :PL) (prods: set Asset): Prop :=
-    set_diff as_dec prods (products_func pl1) = nil.
+    set_diff as_dec prods (products_func pl1) = nil.  
 
   Definition plWeakRefinement_func (pl1 pl2: PL) : Prop :=
     forall p1, set_In p1 (genConf (products_func pl1))->
@@ -95,12 +101,27 @@ Import AssetMappingSPL.
         (assetRef_func (set_add as_dec p1 nil) (set_add as_dec p2 nil)).   
 
   Definition strongerPLrefinement_func (pl1 pl2:PL) : Prop :=
-    forall c1: Conf, set_In c1 (FMRef_Func (getFM_func pl1)) ->
-      (set_In c1 (FMRef_Func (getFM_func pl2)) /\
-          (assetRef_func (CKSem_func (getCK_func pl1) (getAM_func pl1) c1)
-               (CKSem_func (getCK_func pl2) (getAM_func pl2) c1))).
+    forall c, set_In c (FMRef (getFM_func pl1)) ->
+      set_In c (FMRef (getFM_func pl2)) /\
+          (assetRef_func (CKSem (getCK_func pl1) (getAM_func pl1) c)
+               (CKSem (getCK_func pl2) (getAM_func pl2) c)).
 
-  Definition genPL_func (fm: FM) (pl: PL): PL :=
-     ((fm ,(getAM_func pl)), (getCK_func pl)).
+  Definition genPL_func  (fm: FM) (pl: PL) : PL :=
+     {|pls := (fm ,(getAM_func pl), (getCK_func pl)); 
+      wfpl := wfPL_func (fm ,(getAM_func pl), (getCK_func pl)) |}.
+
+  Definition genPLCK_func  (ck: CK) (pl: PL) : PL :=
+     {|pls := ((getFM_func pl) ,(getAM_func pl), ck); 
+      wfpl := wfPL_func ((getFM_func pl) ,(getAM_func pl), ck) |}.
+
+
+  Definition genPLAM_func  (am: AM) (pl: PL) : PL :=
+     {|pls := ((getFM_func pl) ,am, (getCK_func pl)); 
+      wfpl := wfPL_func ((getFM_func pl) ,am, (getCK_func pl)) |}.
+
+  Definition gerPL_func 
+         (fm: FM) (am: AM) (ck: CK): PL :=
+     {|pls := (fm ,am , ck); 
+      wfpl := wfPL_func (fm ,am , ck) |}.
 
 End SPL.
