typeclass/Instances/ckcomp_inst.v
@@ -1,0 +1,115 @@
+Require Export Coq.Lists.ListSet.
+Require Export Coq.Lists.List.
+Require Export Coq.Bool.Bool.
+Require Export Coq.Classes.RelationClasses.
+Require Export maps_def.
+Require Export maps_int.
+Require Export maps_inst.
+Require Export maps_proofs.
+Require Export assettheory_def.
+Require Export formulatheory_def.
+Require Export formulatheory_int.
+Require Export formulatheory_inst.
+Require Export formulatheory_proofs.
+Require Export featuremodelsemantics_def.
+Require Export featuremodelsemantics_int.
+Require Export featuremodelsemantics_inst.
+Require Export assettheory_int.
+Require Export assettheory_inst.
+Require Export ckcomp_int.
+Require Export ckcomp_def.
+Require Export assetmapping_spl_int.
+Require Export assetmapping_spl_def.
+Import AssetMappingSPL.
+Import FormulaTheory.
+Import Maps.
+Import AssetTheory.
+Import FeatureModelSemantics.
+Import CKComp.
+
+
+Program Instance CKComp_Inst : CKComp CK Configuration Formula Item map_ Name AssetName Asset FM :=
+{
+    getExp       := getExp_func;
+    getRS        := getRS_func;
+    exps         := exps_func;
+    SetCompAux   := SetCompAux_func;
+    evalCK       := evalCK_func;
+    assetsCK     := assetsCK_func;
+    imgCK        := imgCK_func;
+    eval         := eval_func;
+    eval2        := eval2_func;
+    notshowupItem:= notshowupItem_func;
+    showupItem   := showupItem_func;
+    semantics_   := semantics_func_;
+    wfCK         := wfCK_func;
+    wfCK2        := wfCK2_func;
+    ckEq         := ckEq_func;
+    ckEq2        := ckEq2_func;
+    renameCKitem := renameCKitem_func;
+    renameCKitem_:= renameCKitem_func_;
+    renamecK     := renamecK_func;
+
+}. Next Obligation.
+{ 
+  apply as_dec_axiom.
+
+} Qed. Next Obligation.
+{
+  apply its_dec_axiom.
+} Qed. Next Obligation.
+{
+  apply its_dec_axiom.
+} Qed. Next Obligation.
+{
+  induction ck.
+  - intros.
+    simpl. reflexivity. 
+  - admit.
+} Admitted. Next Obligation.
+{ admit.
+
+} Admitted. Next Obligation.
+{ 
+  intros. unfold ckEq_func.
+  intros. reflexivity.
+
+} Qed. Next Obligation.
+{
+  unfold ckEq_func. unfold ckEq_func in H. intros. specialize (H c). 
+  intuition.
+} Qed. Next Obligation.
+{
+  unfold ckEq_func. unfold ckEq_func in H. unfold ckEq_func in H0. intros.
+  specialize (H0 c). specialize (H c).
+  intuition. rewrite H2, H. reflexivity.
+} Qed. Next Obligation.
+{
+  unfold ckEq2_func. reflexivity.
+}Qed. Next Obligation.
+{
+  unfold ckEq2_func.   unfold ckEq2_func in H. rewrite H. reflexivity.
+} Qed. Next Obligation.
+{
+  unfold ckEq2_func. unfold ckEq2_func in H. unfold ckEq2_func in H0. 
+  rewrite H, H0. reflexivity.
+} Qed. Next Obligation.
+{
+  unfold not. intros. unfold not in H. apply H.
+  unfold ns_func. unfold wfCK_func in H1. destruct H1. intuition. 
+  admit.
+} Admitted.
+
+
+
+
+
+
+
+
+
+
+
+
+
+
