typeclass/Instances/featuremodelrefinement_inst.v
@@ -1,0 +1,46 @@
+Require Export Coq.Lists.ListSet. 
+Require Export Coq.Classes.SetoidDec.
+Require Export Coq.Lists.List.
+Require Export Coq.Bool.Bool.
+Require Export Coq.Classes.RelationClasses. 
+Require Export featuremodelrefinement_def.
+Require Export featuremodelrefinement_int.
+Import FeatureModelRefinimentTheory.
+Require Export formulatheory_def.
+Require Export formulatheory_proofs.
+Require Export formulatheory_int.
+Import FormulaTheory.
+
+Program Instance FeatureModelRefinement_Ins: FeatureModelRefinement Formula Name FM := 
+{
+  addMandatoryNode:= addMandatoryNode_func;
+  addOptionalNode := addOptionalNode_func;
+
+}. Next Obligation. {
+  apply name_dec_axiom.
+} Qed. Next Obligation. {
+  apply form_dec_axiom.
+} Qed. Next Obligation. {
+  unfold not in H4. unfold ns_func. unfold ns_func in H0, H3, H4, H2.
+  intuition. admit.
+  
+} Admitted. Next Obligation. {
+  unfold FeatureModelSemantics.wfFM_func. split. unfold addMandatoryNode_func in H.
+  destruct H. destruct H0. intuition. admit.
+  admit.
+
+} Admitted. Next Obligation. {
+  admit.
+} Admitted. Next Obligation. {
+  admit.
+} Admitted. Next Obligation. {
+  admit.
+} Admitted. Next Obligation. {
+  admit.
+
+} Admitted. Next Obligation. {
+  admit.
+
+} Admitted.
+
+
