typeclass/Interfaces/ckcomp_int.v
@@ -1,0 +1,92 @@
+Require Export Coq.Lists.ListSet.
+Require Export Coq.Lists.List.
+Require Export Coq.Bool.Bool.
+Require Export Coq.Classes.RelationClasses.
+Require Export assettheory_int.
+Require Export formulatheory_int.
+Require Export maps_int.
+
+
+Class CKComp (Ck Conf FML IT m Nm A N F:Type) {Ft: FormulaTheory FML Nm F} : Type :=
+{
+  (*====================functions=======================*)
+    getExp       : IT -> FML;
+    getRS        : IT -> set A;
+    exps         : list IT -> set FML;
+    SetCompAux   : list IT -> Conf -> set IT;
+    evalCK       : list IT -> Conf -> set IT;
+    assetsCK     : list IT -> set A;
+    imgCK        : list IT -> set A;
+    eval         : list IT -> Conf -> set A;
+    eval2        : list IT -> Conf -> set A;
+    notshowupItem: IT -> A -> Prop;
+    showupItem   : IT -> A -> Prop;
+    semantics_   : list IT -> m -> Conf -> set N;
+    wfCK         : F -> m -> list IT -> Prop;
+    wfCK2        : F -> m -> list IT -> Prop;
+    ckEq         : F -> m -> list IT -> list IT -> Prop;
+    ckEq2        : list IT -> list IT -> Prop;
+    renameCKitem : IT -> A -> A -> IT;
+    renameCKitem_: IT -> Nm -> Nm -> IT;
+    renamecK     : list IT -> Nm -> Nm -> list IT;
+
+  (*===========Axioms - Lemmas - Theorems====================*)
+  as_dec : 
+    forall x y: N, {x = y} + {x <> y};
+  item_dec: 
+    forall x y: IT, {x = y} + {x <> y};
+  ck_dec: 
+    forall x y: IT, {x = y} + {x <> y};
+  lemmaSetComp: forall (ck: list IT) (c: Conf),
+    SetCompAux ck c = set_inter ck_dec ck (SetCompAux ck c);
+  evalUnion: forall (items its1 its2: list IT) (c: Conf) (am: m),
+    items = set_union item_dec its1 its2
+      -> semantics_ items am c = set_union as_dec (semantics_ its1 am c) (semantics_ its2 am c);
+  eqReflexive:
+    forall (fm: F) (am: m) (ck: list IT), ckEq fm am ck ck;
+  eqSymmetric:
+    forall (fm: F) (am: m) (ck1 ck2: list IT), ckEq fm am ck1 ck2 -> ckEq fm am ck2 ck1;
+  eqTransitive:
+    forall (fm: F) (am: m) (ck1 ck2 ck3: list IT),
+      ckEq fm am ck1 ck2 /\ ckEq fm am ck2 ck3 -> ckEq fm am ck1 ck3;
+  eqReflexive2:
+    forall (ck: list IT), ckEq2 ck ck;
+  eqSymmetric2:
+    forall (ck1 ck2: list IT),
+      ckEq2 ck1 ck2 -> ckEq2 ck2 ck1;
+  eqTransitive2:
+    forall (ck1 ck2 ck3: list IT),
+      ckEq2 ck1 ck2 /\ ckEq2 ck2 ck3 -> ckEq2 ck1 ck3;
+  ckNames: forall (fm: F) (am: m) (ck: list IT) (opt: Nm),
+    (
+      (~set_In opt (names_ fm)) /\
+        wfCK fm am ck
+    )
+    ->
+    (forall exp, set_In exp (exps ck) -> (~set_In opt (names exp)))
+
+}.
+
+
+
+
+
+
+
+
+
+
+
+
+
+
+
+
+
+
+
+
+
+
+
+
