typeclass/Interfaces/featuremodelrefinement_int.v
@@ -1,0 +1,65 @@
+Require Import Coq.Lists.ListSet.
+Require Import Coq.Arith.Arith.
+Require Import Coq.Init.Specif.
+Require Export Coq.Lists.List.
+
+
+Require Export formulatheory_int formulatheory_def formulatheory_inst
+               featuremodelsemantics_def featuremodelsemantics_int featuremodelsemantics_inst.
+
+Import  FormulaTheory FeatureModelSemantics.
+
+
+Class FeatureModelRefinement (FML Nm F: Type) {FormT: FormulaTheory FML Nm F} 
+                             {FMS: FeatureModelSemantics FML F Nm }: Type :=
+ {
+  (*====================functions=======================*)
+  addMandatoryNode: F -> F -> Nm -> Nm -> Prop;
+  addOptionalNode : F -> F -> Nm -> Nm -> Prop;
+  
+
+  (*===========Axioms - Lemmas - Theorems====================*)  
+  name_dec : 
+    forall x y: Nm, {x = y} + {x <> y};
+  form_dec : 
+    forall x y: FML, {x = y} + {x <> y};
+  wtFormAddNode: forall (abs con: F) (n1 n2: Nm),
+    wfTree(abs) /\ wfTree(con) /\
+      names_(con) = set_add name_dec n2 (names_ (abs)) /\
+        set_In n1 (names_ (abs)) /\
+          (~set_In n2 (names_ (abs)))
+            -> (forall (f: FML), wt abs f -> wt con f);
+  addMandatoryWF: forall (abs: F) (n1 n2: Nm) (con:F),
+    addMandatoryNode abs con n1 n2 -> wfFM (con);
+  addMandatoryT: forall (abs: F) (n1 n2: Nm),
+    exists (con: F), addMandatoryNode abs con n1 n2 ->
+      (forall (c: set Nm),
+        set_In c (semantics abs)
+          -> if Is_truePB(set_In n1 c) then (set_In (set_add name_dec n2 c) (semantics con))
+            else set_In c (semantics con)) /\
+              (forall (c: set Nm),
+                set_In c (semantics con)
+                  -> if Is_truePB(set_In n2 c) then (set_In (set_remove name_dec n2 c) (semantics abs))
+                    else set_In c (semantics abs)) /\
+                      wfFM(con);
+  addMandatoryTWF: forall (abs: F) (con: F) (n1 n2: Nm),
+  addMandatoryNode abs con n1 n2 ->
+    (forall (c: set Nm),
+      set_In c (semantics abs)
+        -> if Is_truePB(set_In n1 c) then (set_In (set_add name_dec n2 c) (semantics con))
+         else set_In c (semantics con)) /\
+           (forall (c: set Nm),
+              set_In c (semantics con)
+                -> if Is_truePB(set_In n2 c) then (set_In (set_remove name_dec n2 c) (semantics abs))
+                  else set_In c (semantics abs)) /\
+                    wfFM(con);
+  wfPreservation: forall (abs: F) (con: F) (n1 n2: Nm),
+    addOptionalNode abs con n1 n2 -> wfFM (con);
+  addNode: forall (abs: F) (n1 n2: Nm),
+    exists (con: F), addOptionalNode abs con n1 n2 ->
+      refines abs con /\ wfFM con;
+  addOptNode: forall (abs: F) (con: F) (n1 n2: Nm),
+    addMandatoryNode abs con n1 n2 -> 
+     refines abs con /\ wfFM con
+
+}.
