typeclass/Util/ckcomp_def.v
@@ -1,0 +1,128 @@
+Module CKComp.
+
+Require Export Coq.Lists.ListSet.
+Require Export Coq.Lists.List.
+Require Export Coq.Bool.Bool.
+Require Export Coq.Classes.RelationClasses.
+Require Export maps_def.
+Require Export assettheory_def.
+Require Export formulatheory_def.
+Require Export featuremodelsemantics_def.
+Require Export assettheory_int.
+Require Export assettheory_inst.
+Require Export assetmapping_spl_int.
+Require Export assetmapping_spl_def.
+Import AssetMappingSPL.
+Import FormulaTheory.
+Import Maps.
+Import AssetTheory.
+Import FeatureModelSemantics.
+
+  Record Item : Type := {
+  exp: Formula;
+  assets: set AssetName;
+}.
+  Definition CK : Type := list Item.
+  Axiom form_dec_axiom : forall x y:Formula, {x = y} + {x <> y}.
+
+  Variable am am1 am2: AM.
+  Variable  an an1 an2: AssetName.
+  Variable fm: FM.
+  Variable expr: Formula.
+  Variable ck: CK. 
+  Variable item it: Item.
+  Variable items its1 its2: list Item.
+  Variable c c1 c2: Configuration.
+  Variable F G H opt: Name.
+
+  (* get Formula*)
+  Definition getExp_func (it : Item) : Formula := it.(exp).
+  
+  (* get set AssetName*)
+  Definition getRS_func (it: Item) : set AssetName := it.(assets).
+
+   (* Get all Formulas*)
+  Fixpoint exps_func (ck: CK) : set Formula :=
+    match ck with
+    | nil => nil
+    | x :: xs => set_union form_dec_axiom (set_add form_dec_axiom (x.(exp)) nil) (exps_func xs)
+    end.
+
+  Fixpoint SetCompAux_func ck c: set Item :=
+    match ck with
+      | nil => nil
+      | x :: xs => if Is_truePB (satisfies (getExp_func x) c) then
+                   x :: (SetCompAux_func xs c) else (SetCompAux_func xs c)
+    end.
+
+  (*evaluates a CK against a product configuration and
+     yields only CK items evaluated as true *)
+  Definition evalCK_func ck c : set Item := SetCompAux_func ck c.
+
+  (*yields all asset names referenced in a given set of CK items*)
+
+  Fixpoint assetsCK_func (items: list Item): set AssetName :=
+    match items with
+      | nil => nil
+      | x :: xs =>  (x.(assets)) ++ (assetsCK_func xs)
+    end.
+
+  (*  % yields all asset names of a given CK *)
+  Definition imgCK_func ck: set AssetName:=
+    assetsCK_func ck.
+
+  (*yields only the asset names evaluated as true for a given product configuration*)
+  Definition eval_func ck c: set AssetName :=
+    assetsCK_func (evalCK_func ck c).
+
+  (*yields only the asset names evaluated as true for a given product configuration*)
+  Definition eval2_func ck c: set AssetName :=
+    assetsCK_func (evalCK_func ck c).
+
+   Definition notshowupItem_func (it: Item) (an:AssetName) : Prop :=
+    ~ set_In an (it.(assets)).
+  
+  Definition showupItem_func (it: Item) (an:AssetName) : Prop :=
+    set_In an (it.(assets)).
+  
+  Variable a: T.
+
+  (*yields the assets to build a product for a given product configuration 
+   sCK : [ConfigKnowledge->[AM->[Configuration->finite_sets[Asset].finite_set]]] =*)
+  Definition semantics_func_ (ck: CK) (am: AM) (c: Configuration) : set Asset := maps a am (eval_func ck c).
+
+  Axiom as_dec_axiom : forall x y: Asset, {x = y} + {x <> y}.
+  Axiom an_dec_axiom : forall x y: AssetName, {x = y} + {x <> y}.
+  Axiom its_dec_axiom : forall x y: Item, {x = y} + {x <> y}.
+  Axiom ns_dec_axiom : forall x y: Name, {x = y} + {x <> y}.
+
+  Definition wfCK_func fm am ck : Prop :=
+    wfFM_func fm /\ (forall c, set_In c (semantics_func fm) -> (set_diff an_dec_axiom (eval_func ck c) (dom_ am) = nil)) /\
+    (forall exp, set_In exp (exps_func ck) -> wt fm exp).
+
+  Definition wfCK2_func (fm: FM) (am: AM) (ck:CK) : Prop :=
+    (forall item, set_In item ck -> (set_diff an_dec_axiom (item.(assets)) (dom_ am) = nil)) /\
+    (forall exp, set_In exp (exps_func ck) -> wt fm exp).
+
+
+  (* esta vai ser nossa nocao de equivalencia*)
+  Definition ckEq_func (fm: FM) am (ck1 ck2: CK) : Prop :=
+        forall (c: Configuration), set_In c (semantics_func fm) -> ((semantics_func_ ck1 am c) = (semantics_func_ ck2 am c)).
+
+   (*esta vai ser nossa nocao de equivalencia *)
+  Definition ckEq2_func ck1 ck2 : Prop :=
+    eval2_func ck1 = eval2_func ck2.
+
+  Definition renameCKitem_func item (an1 an2: AssetName): Item :=
+    if Is_truePB(set_In an1 (item.(assets))) then item else item.
+
+  Definition renameCKitem_func_ item (F G: Name): Item :=
+    item.
+
+  (*operacao de renaming --> ren: CK x F x F -> CK
+%  renameCK(ck: CK, F,G:Name): set[CKitem] =*)
+
+    Fixpoint renamecK_func (ck: CK) (F G: Name): CK :=
+    nil.
+  
+End CKComp.
