typeclass/Util/featuremodelrefinement_def.v
@@ -1,0 +1,31 @@
+Module FeatureModelRefinimentTheory.
+Require Import Coq.Lists.ListSet.
+Require Import Coq.Arith.Arith.
+Require Import Coq.Init.Specif.
+Require Export Coq.Lists.List.
+
+
+Require Export formulatheory_int formulatheory_def formulatheory_inst
+               featuremodelsemantics_def featuremodelsemantics_int featuremodelsemantics_inst.
+
+Import  FormulaTheory FeatureModelSemantics.
+
+Axiom  name_dec_axiom : 
+    forall x y: Name, {x = y} + {x <> y}.
+Axiom form_dec_axiom : 
+    forall x y: Formula, {x = y} + {x <> y}.
+
+Definition addMandatoryNode_func (abs: FM) (con: FM) (n1 n2: Name): Prop :=
+  fst con = set_add name_dec_axiom n2 (ns_func (abs)) /\
+      snd con = set_union form_dec_axiom (app ((IMPLIES_FORMULA (NAME_FORMULA(n2)) (NAME_FORMULA(n1)))::nil) 
+      ((IMPLIES_FORMULA (NAME_FORMULA(n1)) (NAME_FORMULA(n2)))::nil))
+          (snd abs) /\ set_In n1 (fst abs) /\ (~set_In n2 (fst abs)). 
+
+Definition addOptionalNode_func (abs: FM) (con: FM) (n1 n2: Name): Prop :=
+  fst con = set_add name_dec_axiom n2 (ns_func (abs)) /\ set_In n1 (names_ abs) /\
+     snd con = set_add form_dec_axiom (IMPLIES_FORMULA (NAME_FORMULA(n2)) (NAME_FORMULA(n1)))
+          (snd abs) /\ (~set_In n2 (names_ (abs))).
+
+End FeatureModelRefinimentTheory.
+
+ 
